<?xml version="1.0" encoding="UTF-8" ?>

<!-- ********************************************************************* -->
<!-- Copyright 2017                                                        -->
<!-- Portland Community College                                            -->
<!--                                                                       -->
<!-- Author                                                                -->
<!-- Steve Simonds                                                         -->
<!-- This file is part of PCC SLC Math Resources.                          -->
<!-- ********************************************************************* -->

<section xmlns:xi="http://www.w3.org/2001/XInclude" xml:lang="en-US" xml:id="factoring-binomials">
  <title>Factoring Binomials</title>
  
  <paragraphs>
    <title>Difference of Squares</title>
    <p></p>
  <p>
    A binomial (two term polynomial) of form <m>a^2-b^2</m> always factors into the product
    <m>(a+b)(a-b)</m>.  We can confirm this by applying FOIL to the expression <m>(a+b)(a-b)</m>.
    <md>
      <mrow>(a+b)(a-b)\amp=a^2-ab+ab-b^2</mrow>
      <mrow>\amp=a^2-b^2</mrow>
    </md>
  </p>
  <p>
    A few simple examples follow.  As always, we can check our result by expanding the factored expression.
    <me>x^2-4=(x+2)(x-2)</me><me>y^2-25=(y+5)(y-5)</me><me>36-x^2=(6+x)(6-x)</me>
    Now let's consider a few expressions that don't immediately fit the pattern.  Consider 
    <m>x^{10}-16</m>.  Hopefully we are quick to see that <m>16</m> is the square of <m>4</m>.  To use our factor pattern successfully, we need to also recognize that <m>x^{10}</m> is a perfect square, as is any even power of <m>x</m>.  The power-to-a-power rule of exponents relates that <m>(x^m)^n=x^{mn}</m>.  So the power of <m>x</m> we square that results in <m>x^{10}</m> must be half of <m>10</m>, i.e. <m>5</m>.  Putting it all together we have: <me>x^{10}-16=(x^5+4)(x^5-4)</me> Similar examples follow.
    <me>y^8-9=(y^4+3)(y^4-3)</me><me>x^{46}-1=(x^{23}+1)(x^{23}-1)</me><me>100-w^{12}=(10+w^6)(10-w^6)</me>
  </p>

  <figure xml:id="factoring-geogebra-5">
    <caption>Practice Factoring Difference of Squares with One Variable</caption>
    <interactive platform="geogebra" width="100%" aspect="9:5">
      <slate surface="geogebra" aspect="9:5" source="geogebra/factor-difference-of-squares-basic.ggb">
        setPerspective("G");
        setAxesVisible(0,0);
      </slate>
    </interactive>
  </figure>

   <figure xml:id="factoring-geogebra-6">
    <caption>Practice Factoring Difference of Squares with Two Variables</caption>
    <interactive platform="geogebra" width="100%" aspect="9:5">
      <slate surface="geogebra" aspect="9:5" source="geogebra/factor-difference-of-squares-multivariable.ggb">
        setPerspective("G");
        setAxesVisible(0,0);
      </slate>
    </interactive>
  </figure>
  
  </paragraphs>
  <paragraphs>
    <title>Sum and Difference of Cubes</title>
    <p></p>
  <p>
    A binomial (two term polynomial) of form <m>a^3-b^3</m> always factors into the product <m>(a-b)(a^2+ab+b^2)</m>.  We can confirm this by expanding the expression <m>(a-b)(a^2+ab+b^2)</m>.
    <md>
        <mrow>(a-b)(a^2+ab+b^2)\amp=a^3+a^2b+ab^2-a^2b-ab^2-b^3</mrow>
      <mrow>\amp=a^3-b^3</mrow>
    </md>
  </p>
  <p>
    Similarly, a binomial of form <m>a^3+b^3</m> always factors into the product
  <m>(a+b)(a^2-ab+b^2)</m>.  We can confirm this by expanding the expression <m>(a+b)(a^2-ab+b^2)</m>.
  <md>
    <mrow>(a+b)(a^2-ab+b^2)\amp=a^3-a^2b+ab^2+a^2b-ab^2+b^3</mrow>
    <mrow>\amp=a^3+b^3</mrow>
  </md>
  </p>

  <example xml:id="factoring-binomials-ex-1">
    <statement>
      <p>
        Factor <m>8x^3+27</m> and <m>8x^3-27</m>.
      </p>
    </statement>
    <solution>
      <p>  
        For both binomials, <m>8x^3</m> corresponds to what is identified in the patterns as <m>a^3</m> and <m>27</m> corresponds to what is identified in the pattern as <m>b</m>.  The resultant expressions for <m>a</m>, <m>b</m>, <m>a^2</m>, and <m>b^2</m> and shown in <xref ref="factoring-binomials-table-1">Figure</xref> and the factorizations are shown to the left of the table.
      </p> 
      <sidebyside widths="68% 28%" margins="0%">

        <p>
          <md>
            <mrow>8x^3+27=(2x+3)(4x^2-6x+9)</mrow>
            <mrow></mrow>
            <mrow>8x^3-27=(2x-3)(4x^2+6x+9)</mrow>
          </md>
        </p>

        <figure xml:id="factoring-binomials-table-1">
          <caption></caption>
          <tabular>
            <col halign="center" />
            <col halign="center"/>
            <row>
              <cell>
                <m>a^3=8x^3</m>
              </cell>
              <cell>
                <m>b^3=27</m>
              </cell>
            </row>
            <row>
              <cell><m>a=2x</m></cell>
              <cell><m>b=3</m></cell>
            </row>
            <row>
              <cell><m>a^2=4x^2</m></cell>
              <cell><m>b^2=9</m></cell>
            </row>
            <row>
              <cell><m>ab=6x</m></cell>
            </row>
          </tabular>
        </figure>

      </sidebyside>
    </solution>
  </example>

  <example>
    <statement>
      <p>
        Factor the binomials <m>1+64x^{15}</m> and <m>1-64x^{15}</m>.
      </p>
    </statement>
    <solution>
      <p>
        Note that the power-to-a-power rule of exponents gives us <m>(x^5)^3=x^{(5\times 3)}</m>.
      </p>
      <sidebyside widths="70% 30%" margins="0%">

        <p>
          <md>
            <mrow>1+64x^{15}=(1+4x^5)(1-4x^5+16x^{10})</mrow>
            <mrow></mrow>
            <mrow>1-64x^{15}=(1-4x^5)(1+4x^5+16x^{10})</mrow>
          </md>
        </p>

        <figure xml:id="factoring-binomials-table-2">
          <caption></caption>
          <tabular>
            <col halign="center" />
            <col halign="center"/>
            <row>
              <cell>
                <m>a^3=1</m>
              </cell>
              <cell>
                <m>b^3=64x^{15}</m>
              </cell>
            </row>
            <row>
              <cell><m>a=1</m></cell>
              <cell><m>b=4x^5</m></cell>
            </row>
            <row>
              <cell><m>a^2=1</m></cell>
              <cell><m>b^2=16x^{10}</m></cell>
            </row>
            <row>
              <cell><m>ab=4x^5</m></cell>
            </row>
          </tabular>
        </figure>
      </sidebyside>
    </solution>
  </example>

  <figure xml:id="factoring-geogebra-7">
    <caption>Practice Factoring Sum or Difference of Cubes with one variable</caption>
    <interactive platform="geogebra" width="100%" aspect="9:5">
      <slate surface="geogebra" aspect="9:5" source="geogebra/factor-sum-difference-of-cubes-basic.ggb">
        setPerspective("G");
        setAxesVisible(0,0);
      </slate>
    </interactive>
  </figure>

  <figure xml:id="factoring-geogebra-8">
    <caption>Practice Factoring Sum or Difference of Cubes with two variables</caption>
    <interactive platform="geogebra" width="100%" aspect="9:5">
      <slate surface="geogebra" aspect="9:5" source="geogebra/factor-sum-difference-of-cubes-multivariable.ggb">
        setPerspective("G");
        setAxesVisible(0,0);
      </slate>
    </interactive>
  </figure>

  </paragraphs>
  <paragraphs>
    <title>Sum of Squares</title>
    <p></p>
  <p>
    Unless the expression also happens to be a sum of cubes, sums of squares do not factor - that is, they are prime.                    
  </p>
  <p>
    <m>x^2+4</m> is prime.
  </p>
  <p>
    <m>y^4+25</m> is prime.
  </p>
  <p>
    <m>w^6+4x^2</m> is prime.
  </p>
  <p>
    Many folks would like <m>x^2+4</m> to factor, so much so that they will write <m>x^2+4=(x+2)^2</m>.  Would that it were so.  But alas:
    <md>
      <mrow>(x+2)^2\amp=(x+2)(x+2)</mrow>
      <mrow>\amp=x^2+2x+2x+4</mrow>
      <mrow>\amp=x^2+4x+4</mrow>
    </md>
    In summary, <m>x^2+4\neq (x+2)^2</m>, <m>x^2+4x+4=(x+2)^2</m>.
  </p>
  </paragraphs>

  <exercises>

    <exercisegroup>
      <introduction>
        <p>
          Factor each binomial after first completing the indicated table.
        </p>
      </introduction>

        <exercise>

          <statement>
            <sidebyside widths="70% 30%" margins="0%">

              <p>
                Use the factor pattern <m>a^2-b^2=(a+b)(a-b)</m> to factor <m>x^{10}-25y^4</m> after first completing the entries in <xref ref="factoring-binomials-exercise-table-1">Figure</xref>
              </p>
                      
              <figure xml:id="factoring-binomials-exercise-table-1">
                <caption></caption>
                <tabular>
                  <col halign="center" />
                  <col halign="center"/>
                  <row>
                    <cell>
                      <m>a^2=</m>
                    </cell>
                    <cell>
                      <m>b^2=</m>
                    </cell>
                  </row>
                  <row>
                    <cell><m>a=</m></cell>
                    <cell><m>b=</m></cell>
                  </row>
                </tabular>
              </figure>

            </sidebyside> 
          </statement>

          <solution>
            <sidebyside widths="68% 28%" margins="0%">

              <p>
                <m>x^{10}-25y^4=(x^5+5y^2)(x^5-5y^2)</m> 
              </p>

              <figure xml:id="factoring-binomials-solution-table-1-ans">
                <caption></caption>
                <tabular>
                  <col halign="center" />
                  <col halign="center"/>
                  <row>
                    <cell>
                      <m>a^2=x^{10}</m>
                    </cell>
                    <cell>
                      <m>b^2=25y^4</m>
                    </cell>
                  </row>
                  <row>
                    <cell><m>a=x^5</m></cell>
                    <cell><m>b=5y^2</m></cell>
                  </row>
                  <row>
                    <cell><m>ab=5x^5y^2</m></cell>
                  </row>
                </tabular>
              </figure>
            </sidebyside> 
          </solution>

        </exercise>

        <exercise>

          <statement>
            <sidebyside widths="78% 18%" margins="0%">

              <p>
                Use the factor pattern <m>a^3-b^3=(a-b)(a^2+ab+b^2)</m> to factor <m>8x^3-y^6</m> after first completing the entries in <xref ref="factoring-binomials-exercise-table-2">Figure</xref>
              </p>

              <figure xml:id="factoring-binomials-exercise-table-2">
                <caption></caption>
                <tabular>
                  <col halign="center" />
                  <col halign="center"/>
                  <row>
                    <cell>
                      <m>a^3=</m>
                    </cell>
                    <cell>
                      <m>b^3=</m>
                    </cell>
                  </row>
                  <row>
                    <cell><m>a=</m></cell>
                    <cell><m>b=</m></cell>
                  </row>
                  <row>
                    <cell><m>a^2=</m></cell>
                    <cell><m>b^2=</m></cell>
                  </row>
                  <row>
                    <cell><m>ab=</m></cell>
                  </row>
                </tabular>
              </figure>

            </sidebyside> 
          </statement>
          <solution>
            <sidebyside widths="68% 28%" margins="0%">

              <p>
                <m>8x^3-y^6=(2x-y^2)(4x^2+2xy^2+y^4)</m>
              </p>
                        

              <figure xml:id="factoring-binomials-solution-table-1">
                <caption></caption>
                <tabular>
                  <col halign="center" />
                  <col halign="center"/>
                  <row>
                    <cell>
                      <m>a^3=8x^3</m>
                    </cell>
                    <cell>
                      <m>b^3=y^6</m>
                    </cell>
                  </row>
                  <row>
                    <cell><m>a=2x</m></cell>
                    <cell><m>b=y^2</m></cell>
                  </row>
                  <row>
                    <cell><m>a^2=4x^2</m></cell>
                    <cell><m>b^2=y^4</m></cell>
                  </row>
                  <row>
                    <cell><m>ab=2xy^2</m></cell>
                  </row>
                </tabular>
              </figure>
            </sidebyside> 
          </solution>

        </exercise>

        <exercise>
          <statement>
            <sidebyside widths="78% 18%" margins="0%">

              <p>
                Use the factor pattern <m>a^3+b^3=(a+b)(a^2-ab+b^2)</m> to factor <m>125t^{12}+27x^9</m> after first completing the entries in <xref ref="factoring-binomials-exercise-table-3">Figure</xref>
              </p>

              <figure xml:id="factoring-binomials-exercise-table-3">
                <caption></caption>
                <tabular>
                  <col halign="center" />
                  <col halign="center"/>
                  <row>
                    <cell>
                      <m>a^3=</m>
                    </cell>
                    <cell>
                      <m>b^3=</m>
                    </cell>
                  </row>
                  <row>
                    <cell><m>a=</m></cell>
                    <cell><m>b=</m></cell>
                  </row>
                  <row>
                    <cell><m>a^2=</m></cell>
                    <cell><m>b^2=</m></cell>
                  </row>
                  <row>
                    <cell><m>ab=</m></cell>
                  </row>
                </tabular>
              </figure>

            </sidebyside>  
          </statement>
          <solution>
            <sidebyside widths="38% 58%" margins="0%">
              <figure xml:id="factoring-binomials-solution-table-3">
                <caption></caption>
                <tabular>
                  <col halign="center" />
                  <col halign="center"/>
                  <row>
                    <cell>
                      <m>a^3=125t^{12}</m>
                    </cell>
                    <cell>
                      <m>b^3=27x^9</m>
                    </cell>
                  </row>
                  <row>
                    <cell><m>a=5t^4</m></cell>
                    <cell><m>b=3x^3</m></cell>
                  </row>
                  <row>
                    <cell><m>a^2=25t^8</m></cell>
                    <cell><m>b^2=9x^6</m></cell>
                  </row>
                  <row>
                    <cell><m>ab=15t^4x^3</m></cell>
                  </row>
                </tabular>
              </figure>

              <p>
              </p>
            </sidebyside>
            <p>
              <m>125t^{12}+27x^9=(5t^4+3x^3)(25t^8-15t^4x^3+9x^6)</m>
            </p>
          </solution>

        </exercise>

      </exercisegroup>

      <exercisegroup>
        <introduction>
          <p>
                    Factor each binomial.  Check your result by expanding the factored expression.  If the binomial does not factor, state that it is prime.
          </p>
        </introduction>

        <exercise>
          <statement>
            <p>
              <m>36p^2-q^2</m>
            </p>
          </statement>
          <solution>
            <p>
              <m>36p^2-q^2=(6p+q)(6p-q)</m>
            </p>
          </solution>
        </exercise>

        <exercise>
          <statement>
            <p>
              <m>36p^2+q^2</m>
            </p>
          </statement>
          <solution>
            <p>
              <m>36p^2+q^2 </m> is prime.
            </p>
          </solution>
        </exercise>

        <exercise>
          <statement>
            <p>
              <m>125+y^3</m>
            </p>
          </statement>
          <solution>
            <p>
              <m>125+y^3=(5+y)(25-5y+y^2)</m>
            </p>
          </solution>
        </exercise>

        <exercise>
          <statement>
            <p>
              <m>8x^3-27y^3</m>
            </p>
          </statement>
          <solution>
            <p>
              <m>8x^3-27y^3=(2x-3y)(4x^2+6xy+9y^2)</m>
            </p>
          </solution>
        </exercise>

      </exercisegroup>

    </exercises>

  </section>
