<?xml version="1.0" encoding="UTF-8" ?>

<!-- ********************************************************************* -->
<!-- Copyright 2017                                                        -->
<!-- Portland Community College                                            -->
<!--                                                                       -->
<!-- Author                                                                -->
<!-- Steve Simonds                                                         -->
<!-- This file is part of PCC SLC Math Resources.                          -->
<!-- ********************************************************************* -->

<section xmlns:xi="http://www.w3.org/2001/XInclude" xml:lang="en-US" xml:id="section-workshop-simplifying-expressions-containing-square-roots">
    <title>Simplifying expressions containing square roots</title>

    <exercises>
    <title>Pretest - what's your current skill set?</title>

        
  </exercises>

  <exercises>
    <title>Written Examples</title>

    

       
  </exercises>

 <exercises>
    <title>Practice Exercises</title>

     <exercise xml:id="workshop-radicals-and-rat-exp-simplify-sq-rt-exercises">
      <title>Simplifying square roots by factoring out perfect squares</title>
      <statement>
        <p>
          Simplify each square root expression.
          <ol cols="3">
            <li><m>\sqrt{50}</m></li>
            <li><m>\sqrt{20}</m></li>
            <li><m>\sqrt{27}</m></li>
            <li><m>5\sqrt{72}</m></li>
            <li><m>\frac{\sqrt{8}}{2}</m></li>
            <li><m>-9\sqrt{12}</m></li>
          </ol>
          <p>
          </p>
        </p>
      </statement>

      <solution>
        <p>
          <ol cols="2">

            <li>
              <m>
                \begin{aligned}[t]
                \sqrt{50}\amp=\sqrt{25 \cdot 2}\\
                \amp=\sqrt{25} \cdot \sqrt{2}\\
                \amp=5\sqrt{2}
                \end{aligned}
              </m>
            </li>

            <li>
              <m>
                \begin{aligned}[t]
                \sqrt{20}\amp=\sqrt{4 \cdot 5}\\
                \amp=\sqrt{4} \cdot \sqrt{5}\\
                \amp=2\sqrt{5}
                \end{aligned}
              </m>
            </li>

            <li>
              <m>
                \begin{aligned}[t]
                \sqrt{27}\amp=\sqrt{9 \cdot 3}\\
                \amp=\sqrt{9} \cdot \sqrt{3}\\
                \amp=3\sqrt{3}
                \end{aligned}
              </m>
            </li>

            <li>
              <m>
                \begin{aligned}[t]
                5\sqrt{72}\amp=5 \cdot \sqrt{36 \cdot 2}\\
                \amp=5 \cdot \sqrt{36} \cdot \sqrt{2}\\
                \amp=5 \cdot 6 \cdot \sqrt{2}\\
                \amp=30\sqrt{2}
                \end{aligned}
              </m>
            </li>

            <li>
              <m>
                \begin{aligned}[t]
                \frac{\sqrt{8}}{2}\amp=\frac{\sqrt{4 \cdot 2}}{2}\\
                \amp=\frac{\sqrt{4} \cdot \sqrt{2}}{2}\\
                \amp=\frac{2 \cdot \sqrt{2}}{2}\\
                \amp=\sqrt{2}
                \end{aligned}
              </m>
            </li>

            <li>
              <m>
                \begin{aligned}[t]
                -9\sqrt{12}\amp=-9 \cdot \sqrt{4 \cdot 3}\\
                \amp=-9\sqrt{4} \cdot \sqrt{3}\\
                \amp=-9 \cdot 2 \cdot \sqrt{3}\\
                \amp=-18\sqrt{3}
                \end{aligned}
              </m>
            </li>

          </ol>
        </p>
      </solution>

    </exercise>

 
    <exercise xml:id="workshop-radicals-and-rat-exp-mono-sq-rt-exercises">
      <title>Rationalizing monomial square root denominators</title>
      <statement>
        <p>
          Rationalize each denominator.  Completely simplify each result.
          <ol cols="3">
            <li><m>\frac{7}{\sqrt{7}}</m></li>
            <li><m>\frac{30}{\sqrt{10}}</m></li>
            <li><m>\frac{1}{\sqrt{20}}</m></li>
            <li><m>\frac{25}{\sqrt{50}}</m></li>
            <li><m>\frac{1}{6\sqrt{3}}</m></li>
            <li><m>\frac{121}{11\sqrt{11}}</m></li>
          </ol>
          <p>
          </p>
        </p>
      </statement>
      <solution>
        <ol cols="2">

          <li>
            <m>
              \begin{aligned}[t]
              \frac{7}{\sqrt{7}}\amp=\frac{7}{\sqrt{7}} \cdot \frac{\sqrt{7}}{\sqrt{7}}\\
              \amp=\frac{7\sqrt{7}}{7}\\
              \amp=\sqrt{7}
              \end{aligned}
            </m>
          </li>

          <li>
            <m>
              \begin{aligned}[t]
              \frac{30}{\sqrt{10}}\amp=\frac{30}{\sqrt{10}} \cdot \frac{\sqrt{10}}{\sqrt{10}}\\
              \amp=\frac{30\sqrt{10}}{10}\\
              \amp=3\sqrt{10}
              \end{aligned}
            </m>
          </li>

          <li>
            <m>
              \begin{aligned}[t]
              \frac{1}{\sqrt{20}}\amp=\frac{1}{\sqrt{20}} \cdot \frac{\sqrt{20}}{\sqrt{20}}\\
              \amp=\frac{\sqrt{20}}{20}\\
              \amp=\frac{2\sqrt{5}}{20}\\
              \amp=\frac{\sqrt{5}}{10}
              \end{aligned}
            </m>
          </li>

          <li>
            <m>
              \begin{aligned}[t]
              \frac{25}{\sqrt{50}}\amp=\frac{25}{\sqrt{50}} \cdot \frac{\sqrt{50}}{\sqrt{50}}\\
              \amp=\frac{25\sqrt{50}}{50}\\
              \amp=\frac{\sqrt{50}}{2}\\
              \amp=\frac{5\sqrt{2}}{2}
              \end{aligned}
            </m>
          </li>

          <li>
            <m>
              \begin{aligned}[t]
              \frac{1}{6\sqrt{3}}\amp=\frac{1}{6\sqrt{3}} \cdot \frac{\sqrt{3}}{\sqrt{3}}\\
              \amp=\frac{\sqrt{3}}{6 \cdot 3}\\
              \amp=\frac{\sqrt{3}}{18}
              \end{aligned}
            </m>
          </li>

          <li>
            <m>
              \begin{aligned}[t]
              \frac{121}{11\sqrt{11}}\amp=\frac{121}{11\sqrt{11}} \cdot \frac{\sqrt{11}}{\sqrt{11}}\\
              \amp=\frac{121\sqrt{11}}{11 \cdot 11}\\
              \amp=\sqrt{11}
              \end{aligned}
            </m>
          </li>


        </ol>
      </solution>
    </exercise>

     <exercise xml:id="workshop-radicals-and-rat-exp-add-sq-rt-exercises">
      <title>Combining square root expressions</title>
      <statement>
        <p>
          Combine all like terms after first simplifying each term containing a square root.
          <ol cols="2">
            <li><m>\sqrt{2}+\sqrt{8}</m></li>
            <li><m>\sqrt{9}+\sqrt{18}</m></li>
            <li><m>4\sqrt{12}-7\sqrt{18}</m></li>
            <li><m>(\sqrt{6}+\sqrt{2})^2</m></li>
            <li><m>(\sqrt{8}+2)(\sqrt{8}-2)</m></li>
            <li><m>5\sqrt{12}+\frac{6}{\sqrt{3}}</m></li>
            <p>
            </p>
          </ol>
          <p>
          </p>
        </p>
      </statement>
      <solution>
        <p>
          <ol>

            <li>
              <m>
                \begin{aligned}[t]
                \sqrt{2}+\sqrt{8}\amp=\sqrt{2}+2\sqrt{2}\\
                \amp=3\sqrt{2}              
                \end{aligned}
              </m>
            </li>

            <li>
              <m>
                \begin{aligned}[t]
                \sqrt{9}+\sqrt{18}=3+3\sqrt{2}              
                \end{aligned}
              </m>
            </li>

            <li>
              <m>
                \begin{aligned}[t]
                4\sqrt{8}-7\sqrt{18}\amp=4 \cdot 2\sqrt{2}-7 \cdot 3\sqrt{2}\\
                \amp=8\sqrt{2}-21\sqrt{2}\\
                \amp=-13\sqrt{2}
                \end{aligned}
              </m>
            </li>

           

            <li>
              <m>
                \begin{aligned}[t]
                (\sqrt{6}+\sqrt{2})^2\amp=(\sqrt{6}+\sqrt{2})(\sqrt{6}+\sqrt{2})\\
                \amp=6+\sqrt{12}+\sqrt{12}+2\\
                \amp=6+2\sqrt{3}+2\sqrt{3}+2\\
                \amp=8+4\sqrt{3}              
                \end{aligned}
              </m>
            </li>

            <li>
              <m>
                \begin{aligned}[t]
                (\sqrt{8}+2)(\sqrt{8}-2)\amp=8-2\sqrt{8}+2\sqrt{8}-4\\
                \amp=4              
                \end{aligned}
              </m>
            </li>

            <li>
              <m>
                \begin{aligned}[t]
                5\sqrt{12}+\frac{6}{\sqrt{3}}\amp=5 \cdot 2\sqrt{3}+\frac{6}{\sqrt{3}} \cdot \frac{\sqrt{3}}{\sqrt{3}}\\
                \amp=10\sqrt{3}+2\sqrt{3}\\
                \amp=12\sqrt{3}              
                \end{aligned}
              </m>
            </li>
          
          </ol>
        </p>
      </solution>

    </exercise>


    <exercise xml:id="workshop-radicals-and-rat-exp-rat-bi-den-exercises">
      <title>Rationalizing binomial denominators containing square root expressions</title>

      <statement>
        <p>
          Rationalize each denominator.  Completely simplify each result.
          <ol cols="2">
            <li><m>\frac{7}{3-\sqrt{2}}</m></li>
            <li><m>\frac{5}{\sqrt{7}+\sqrt{2}}</m></li>
            <li><m>\frac{8}{\sqrt{12}+4}</m></li>
            <li><m>\frac{\sqrt{3}+\sqrt{2}}{\sqrt{3}-\sqrt{2}}</m></li>
            <li><m>\frac{\sqrt{8}}{\sqrt{2}+\sqrt{3}}</m></li>
          </ol>
          <p>
          </p>
        </p>
      </statement>

      <solution>
        <ol>

          <li>
            <m>
              \begin{aligned}[t]
              \frac{7}{3-\sqrt{2}}\amp=\frac{7}{3-\sqrt{2}} \cdot \frac{3+\sqrt{2}}{3+\sqrt{2}}\\
              \amp=\frac{7(3+\sqrt{2})}{9-2}\\
              \amp=\frac{7(3+\sqrt{2})}{7}\\
              \amp=3+\sqrt{2}
              \end{aligned}
            </m>            
          </li>

           <li>
            <m>
              \begin{aligned}[t]
              \frac{5}{\sqrt{7}+\sqrt{2}}\amp=\frac{5}{\sqrt{7}+\sqrt{2}} \cdot \frac{\sqrt{7}-\sqrt{2}}{\sqrt{7}-\sqrt{2}}\\
              \amp=\frac{5(\sqrt{7}-\sqrt{2})}{7-2}\\
              \amp=\frac{5(\sqrt{7}-\sqrt{2})}{5}\\
              \amp=\sqrt{7}-\sqrt{2}
              \end{aligned}
            </m>            
          </li>

           <li>
            <m>
              \begin{aligned}[t]
              \frac{8}{\sqrt{12}+4}\amp=\frac{8}{\sqrt{12}+4} \cdot \frac{\sqrt{12}-4}{\sqrt{12}-4}\\
              \amp=\frac{8(\sqrt{12}-4)}{12-16}\\
              \amp=\frac{8(\sqrt{12}-4)}{-4}\\
              \amp=-2(\sqrt{12}-4)\\
              \amp=-2(2\sqrt{3}-4)\\
              \amp=-4\sqrt{3}+16
              \end{aligned}
            </m>            
          </li>

           <li>
            <m>
              \begin{aligned}[t]
              \frac{\sqrt{3}+\sqrt{2}}{\sqrt{3}-\sqrt{2}}\amp=\frac{\sqrt{3}+\sqrt{2}}{\sqrt{3}-\sqrt{2}} \cdot \frac{\sqrt{3}+\sqrt{2}}{\sqrt{3}+\sqrt{2}}\\
              \amp=\frac{3+\sqrt{6}+\sqrt{6}+2}{3-2}\\
              \amp=5+2\sqrt{6}
              \end{aligned}
            </m>            
          </li>

           <li>
            <m>
              \begin{aligned}[t]
              \frac{\sqrt{8}}{\sqrt{2}+\sqrt{3}}\amp=\frac{\sqrt{8}}{\sqrt{2}+\sqrt{3}} \cdot \frac{\sqrt{2}-\sqrt{3}}{\sqrt{2}-\sqrt{3}}\\
              \amp=\frac{\sqrt{8}(\sqrt{2}-\sqrt{3})}{2-3}\\
              \amp=\frac{\sqrt{16}-\sqrt{24}}{-1}\\
              \amp=-(4-2\sqrt{6})\\
              \amp=-4+2\sqrt{6}
              \end{aligned}
            </m>            
          </li>

        </ol>
      </solution>
    </exercise>

   
  </exercises>


   

     
</section>
