<?xml version="1.0" encoding="UTF-8" ?>

<!-- ********************************************************************* -->
<!-- Copyright 2017                                                        -->
<!-- Portland Community College                                            -->
<!--                                                                       -->
<!-- Author                                                                -->
<!-- Steve Simonds                                                         -->
<!-- This file is part of PCC SLC Math Resources.                          -->
<!-- ********************************************************************* -->

<section xmlns:xi="http://www.w3.org/2001/XInclude" xml:lang="en-US" xml:id="section-workshop-radicals-and-rational-exponents">
    <title>Radicals and rational exponents</title>

    <exercises>
      <title>Written Examples</title>

     <exercise>
      <title>Converting between radical notation and rational exponent notation</title>
      <statement>
        <p>
          The power to a power rule of exponents states that <m>(x^m)^n=x^{mn}</m>.  This rule is fairly intuitive when both exponents are positive.  For example, in the expression <m>(x^4)^3</m> there are three factors of <m>x^4</m>, each of which contains four factors of <m>x</m>, so all together there are four factors of <m>x</m>, three times, i.e. <m>3 \cdot 4</m> factor of <m>x</m>.
        </p>
        <p>
          While the power to a power rule is less intuitive once you move away from positive integer exponents, the rule remains the same regardless of the nature of the exponents.  For example:
          <md>
            <mrow>(x^{1/3})^3\amp=x^{\frac{1}{3} \cdot 3}</mrow>
            <mrow>\amp=x^{1}</mrow>
            <mrow>\amp=x</mrow>
          </md>
          But we already have a name for the expression that when cubed results in <m>x</m>, and that name is <m>\sqrt[3]{x}</m> (the cube root of <m>x</m>).  So it must be the case that <m>x^{1/3}=\sqrt[3]{x}</m>.  In general, is <m>n</m> is any positive integer, then: <me>x^{1/n}=\sqrt[n]{x}</me> and more generally, <me>x^{m/n}=\sqrt[n]{x^m}</me>.
        </p>
        Several examples are shown below.
        <sidebyside widths="33% 33% 33%" margins="0%">
          <p>
            <me>y^{7/5}=\sqrt[5]{y^7}</me>
          </p>
          <p>
            <md>
              <mrow>\sqrt[3]{w^{12}}\amp=w^{12/3}</mrow>
              <mrow>\amp=w^4</mrow>
            </md>
          </p>
          <p>
            <me>\sqrt{x^9}=x^{9/2}</me>
          </p>
        </sidebyside>
      </statement>
    </exercise>

    <exercise>
      <title>Evaluating expressions that include rational exponents</title>
      <statement>
        <p>
          As long as both the numerator and denominator of a rational exponent are fairly small positive numbers, it is fairly easy to evaluate expressions that include rational exponents using the rule <m>x^{m/n}=\sqrt[n]{x^m}</m>.  For example:
          <sidebyside widths="33% 33% 33%" margins="0%">
            <p>
              <md>
                <mrow>16^{1/2}\amp=\sqrt{16}</mrow>
                <mrow>\amp=4</mrow>
              </md>
            </p>
            <p>
              <md>
                <mrow>8^{2/3}\amp=\sqrt[3]{8^2}</mrow>
                <mrow>\amp=\sqrt[3]{64}</mrow>
                <mrow>\amp=4</mrow>
              </md>
            </p>
            <p>
              <md>
                <mrow>100^{3/2}\amp=\sqrt{100^3}</mrow>
                <mrow>\amp=\sqrt{1000000}</mrow>
                <mrow>\amp=1000</mrow>
              </md>
            </p>
          </sidebyside>
        </p>
        <p>When the numerator of the rational exponent is large, the rule <m>x^{m/n}=\sqrt[n]{x^m}</m> can become quite cumbersome.  Consider, for example, evaluating <m>9^{5/2}</m>.  If we try to use the standard form we hit a brick wall.  First, it's not trivial to calculate that <m>9^5=59,049</m> (reality check ... I grabbed my calculator).  Now that I have the value of 59,049, I have to determine its square root.  Oh my!
        </p>
        <p>
          Fortunately for us, the application of the exponent and the application of the radical can be done in either order.  That is:
        </p>
        <p>
          <me>a^{m/n}=\sqrt[n]{x^m}   \text{  and  }   a^{m/n}=(\sqrt[n]{x})^m</me>
        </p>
        <p>
          Using the second option, evaluation of <m>9^{5/2}</m> becomes much less daunting.
          <md>
            <mrow>9^{5/2}\amp=(\sqrt{9})^5</mrow>
            <mrow>\amp=3^5</mrow>
            <mrow>\amp=243</mrow>
          </md>
        </p>
        <p>
          Similarly:
          <md>
            <mrow>16^{7/4}\amp=(\sqrt[4]{16})^7</mrow>
            <mrow>\amp=2^7</mrow>
            <mrow>\amp=128</mrow>
          </md>
        </p>
        <p>
          Although you might prefer it not to be, rational exponents are allowed to be negative.  If that's the case, you probably want to deal with the negative aspect of the exponent before taking on the fractional aspect.  For example:
        <md>
          <mrow>27^{-2/3}\amp=\frac{1}{27^{2/3}}</mrow>
          <mrow>\amp=\frac{1}{(\sqrt[3]{27})^2}</mrow>
          <mrow>\amp=\frac{1}{3^2}</mrow>
          <mrow>\amp=\frac{1}{9}</mrow>
        </md>
      </p>
      </statement>
    </exercise>

    <exercise>
      <title>Using rational exponents to simplify radical expressions</title>
      <statement>
        <p>
          Sometimes radical expressions can be simplified after first rewriting the expressions using rational exponents and applying the appropriate rules of exponents.  If the resultant expression still has a rational exponent, it is standard to convert back to radical notation.  Several examples follow.
        </p>
        <sidebyside widths="33% 33% 33%" margins="0%">
          <p>
            <md>
              <mrow>\sqrt[3]{y^2} \cdot \sqrt[6]{y}\amp=y^{2/3}y^{1/6}</mrow>
              <mrow>\amp=y^{2/3+1/6}</mrow>
              <mrow>\amp=y^{5/6}</mrow>
              <mrow>\amp=\sqrt[6]{y^5}</mrow>
            </md>
          </p>
          <p>
            <md>
              <mrow>\sqrt[8]{t^4}\amp=t^{4/8}</mrow>
              <mrow>\amp=t^{1/2}</mrow>
              <mrow>\amp=\sqrt{t}</mrow>
            </md>
          </p>
          <p>
            <md>
              <mrow>\sqrt[10]{\sqrt{5^{40}}}\amp=\sqrt[10]{5^{40/2}}</mrow>
              <mrow>\amp=\sqrt[10]{5^{20}}</mrow>
              <mrow>\amp=5^{20/10}</mrow>
              <mrow>\amp=5^2</mrow>
              <mrow>\amp=25</mrow>
            </md>
          </p>
        </sidebyside>
      </statement>
    </exercise>

  </exercises>

  <exercises>
      <title>Practice Exercises</title>

    <exercise>
      <title>Converting between radical notation and rational exponent notation</title>
      <statement>
        <p>
          Convert each exponent expression to a radical expression and each radical expression to an exponent expression.  Assume that all variables represent positive values.
          <ol cols="3">
            <li><m>x^{1/3}</m></li>
            <li><m>y^{5/4}</m></li>
            <li><m>z^{2/5}</m></li>
            <li><m>\sqrt[11]{x^5}</m></li>
            <li><m>\sqrt[4]{y^{20}}</m></li>
            <li><m>\sqrt[15]{t^3}</m></li>
          </ol>
          <p>
          </p>
        </p>
      </statement>

      <solution>
        <p>
          <ol cols="2">
            <li><m>x^{1/3}=\sqrt[3]{x}</m></li>
            <li><m>y^{5/4}=\sqrt[4]{y^5}</m></li>
            <li><m>z^{2/5}=\sqrt[5]{z^2}</m></li>
            <li><m>\sqrt[11]{x^5}=x^{5/11}</m></li>

            <li>
              <m>
                \begin{aligned}[t]
                \sqrt[4]{y^{20}}\amp=y^{20/4}\\
                \amp=y^5
                \end{aligned}
              </m>            
            </li>

            <li>
              <m>
                \begin{aligned}[t]
                \sqrt[15]{t^3}\amp=t^{3/15}\\
                \amp=t^{1/5}
                \end{aligned}
              </m>            
            </li>

          </ol>
        </p>
      </solution>

    </exercise>

    <exercise>
      <title>Evaluating expressions that include rational exponents</title>
      <statement>
        <p>
          Determine the value of each expression.
          <ol cols="3">
            <li><m>4^{1/2}</m></li>
            <li><m>27^{-1/3}</m></li>
            <li><m>(\frac{4}{9})^{-1/2}</m></li>
            <li><m>8^{7/3}</m></li>
            <li><m>100^{5/2}</m></li>
            <li><m>16^{-9/4}</m></li>
          </ol>
          <p>
          </p>
        </p>
      </statement>

      <solution>
        <ol cols="2">

          <li>
            <m>
              \begin{aligned}[t]
              4^{1/2}\amp=\sqrt{4}\\
              \amp=2
              \end{aligned}
            </m>            
          </li>

          <li>
            <m>
              \begin{aligned}[t]
              27^{-1/3}\amp=\frac{1}{27^{1/3}}\\
              \amp=\frac{1}{\sqrt[3]{27}}\\
              \amp=\frac{1}{3}
              \end{aligned}
            </m>            
          </li>

          <li>
            <m>
              \begin{aligned}[t]
              (\frac{4}{9})^{-1/2}\amp=(\frac{9}{4})^{1/2}\\
              \amp=\sqrt{\frac{9}{4}}\\
              \amp=\frac{3}{2}
              \end{aligned}
            </m>            
          </li>

          <li>
            <m>
              \begin{aligned}[t]
              8^{7/3}\amp=(\sqrt[3]{8})^7\\
              \amp=2^7\\
              \amp=128
              \end{aligned}
            </m>            
          </li>

          <li>
            <m>
              \begin{aligned}[t]
              100^{5/2}\amp=(\sqrt{100})^5\\
              \amp=10^5\\
              \amp=100,000
              \end{aligned}
            </m>            
          </li>

          <li>
            <m>
              \begin{aligned}[t]
              16^{-9/4}\amp=\frac{1}{16^{9/4}}\\
              \amp=\frac{1}{(\sqrt[4]{16})^9}\\
              \amp=\frac{1}{2^9}\\
              \amp=\frac{1}{512}
              \end{aligned}
            </m>            
          </li>

        </ol>
      </solution>
    </exercise>

    <exercise>
      <title>Using rational exponents to simplify radical expressions</title>
      <statement>
        <p>
          Simplify each radical expression after first rewriting the expression in exponential form.  Assume that all variables represent positive values.
          <ol cols="3">
            <li><m>\sqrt[5]{t^{20}}</m></li>
            <li><m>6\sqrt[33]{x^{77}}</m></li>
            <li><m>(\sqrt{3})^{10}</m></li>
            <li><m>\sqrt[4]{9^2}</m></li>
            <li><m>\sqrt{w}\sqrt[4]{w}</m></li>
            <li><m>\sqrt[7]{x^6}\sqrt[7]{x}</m></li>
            <li><m>(\sqrt[12]{x^7y^{16}})^{36}</m></li>
            <li><m>\sqrt[5]{\sqrt[3]{x^{15}}}</m></li>
          </ol>
          <p>
          </p>
        </p>
      </statement>

      <solution>
        <p>
          <ol cols="2">

            <li>
              <m>
                \begin{aligned}[t]
                \sqrt[5]{t^{20}}\amp=t^{20/5}\\
                \amp=t^4
                \end{aligned}
              </m>            
            </li>

            <li>
              <m>
                \begin{aligned}[t]
                6\sqrt[33]{x^{77}}\amp=6x^{77/33}\\
                \amp=6x^{7/3}\\
                \amp=6\sqrt[3]{x^7}
                \end{aligned}
              </m>            
            </li>

            <li>
              <m>
                \begin{aligned}[t]
                (\sqrt{3})^{10}\amp=3^{10/2}\\
                \amp=3^5\\
                \amp=243
                \end{aligned}
              </m>            
            </li>

            <li>
              <m>
                \begin{aligned}[t]
                \sqrt[4]{9^2}\amp=9^{2/4}\\
                \amp=9^{1/2}\\
                \amp=\sqrt{9}\\
                \amp=3
                \end{aligned}
              </m>            
            </li>

            <li>
              <m>
                \begin{aligned}[t]
                \sqrt{w}\sqrt[4]{w}\amp=w^{1/2}w^{1/4}\\
                \amp=w^{3/4}\\
                \amp=\sqrt[4]{w^3}
                \end{aligned}
              </m>            
            </li>

            <li>
              <m>
                \begin{aligned}[t]
                \sqrt[7]{x^6}\sqrt[7]{x}\amp=x^{6/7}x^{1/7}\\
                \amp=x^1\\
                \amp=x
                \end{aligned}
              </m>            
            </li>

            <li>
              <m>
                \begin{aligned}[t]
                (\sqrt[12]{x^7y^{15}})^{36}\amp=(x^7y^{16})^{36/12}\\
                \amp=(x^7y^{16})^3\\
                \amp=x^{21}y^{48}
                \end{aligned}
              </m>            
            </li>

            <li>
              <m>
                \begin{aligned}[t]
                \sqrt[15]{\sqrt[3]{x^{15}}}\amp=\sqrt[15]{x^{15/3}}\\
                \amp=\sqrt[15]{x^5}\\
                \amp=x^{5/15}\\
                \amp=x^{1/3}\\
                \amp=\sqrt[3]{x}

                \end{aligned}
              </m>            
            </li>

          </ol>
        </p>
      </solution>
    </exercise>

  </exercises>
   

     
</section>
